Stack example

examples/stack/Stack1.v
@@ -19,8 +19,8 @@ Section PROOF.
   Context `{Σ: GRA.t}.
   Context `{@GRA.inG memRA Σ}.
 
-  Notation pget := (p0 <- trigger PGet;; `p0: (gmap mblock (list val)) <- p0↓ǃ;; Ret p0) (only parsing).
-  Notation pput p0 := (trigger (PPut (p0: (gmap mblock (list val)))↑)) (only parsing).
+  Notation sget := (p0 <- trigger sGet;; `p0: (gmap mblock (list val)) <- p0↓ǃ;; Ret p0) (only parsing).
+  Notation sput p0 := (trigger (sPut (p0: (gmap mblock (list val)))↑)) (only parsing).
 
   (* def new(): Ptr *)
   (*   let handle := Choose(Ptr); *)
@@ -32,10 +32,10 @@ Section PROOF.
     fun args =>
       _ <- (pargs [] args)?;;;
       handle <- trigger (Choose _);;;
-      stk_mgr0 <- pget;;;
+      stk_mgr0 <- sget;;;
       guarantee(stk_mgr0 !! handle = None);;;
       let stk_mgr1 := <[handle:=[]]> stk_mgr0 in
-      _ <- pput stk_mgr1;;;
+      _ <- sput stk_mgr1;;;
       Ret (Vptr handle 0)
   .
 
@@ -51,15 +51,15 @@ Section PROOF.
   Definition pop_body: list val -> itree hEs val :=
     fun args =>
       handle <- (pargs [Tblk] args)?;;;
-      stk_mgr0 <- pget;;;
+      stk_mgr0 <- sget;;;
       stk0 <- (stk_mgr0 !! handle)?;;;
-      let stk_mgr1 := delete handle stk_mgr0 in _ <- pput stk_mgr1;;;
+      let stk_mgr1 := delete handle stk_mgr0 in _ <- sput stk_mgr1;;;
       match stk0 with
       | x :: stk1 =>
-        stk_mgr2 <- pget;;; _ <- pput (<[handle:=stk1]> stk_mgr2);;;
+        stk_mgr2 <- sget;;; _ <- sput (<[handle:=stk1]> stk_mgr2);;;
         Ret x
       | _ =>
-        stk_mgr2 <- pget;;; _ <- pput (<[handle:=[]]> stk_mgr2);;;
+        stk_mgr2 <- sget;;; _ <- sput (<[handle:=[]]> stk_mgr2);;;
         Ret (Vint (- 1))
       end
   .
@@ -72,45 +72,45 @@ Section PROOF.
   Definition push_body: list val -> itree hEs val :=
     fun args =>
       '(handle, x) <- (pargs [Tblk; Tuntyped] args)?;;;
-      stk_mgr0 <- pget;;;
+      stk_mgr0 <- sget;;;
       stk0 <- (stk_mgr0 !! handle)?;;;
-      let stk_mgr1 := delete handle stk_mgr0 in _ <- pput stk_mgr1;;;
-      stk_mgr2 <- pget;; pput (<[handle:=(x :: stk0)]> stk_mgr2);;;
+      let stk_mgr1 := delete handle stk_mgr0 in _ <- sput stk_mgr1;;;
+      stk_mgr2 <- sget;; sput (<[handle:=(x :: stk0)]> stk_mgr2);;;
       Ret Vundef
   .
 
-  Definition StackSbtb: list (gname * kspecbody) :=
-    [("new", ksb_trivial (cfunU new_body));
-    ("pop", ksb_trivial (cfunU pop_body));
-    ("push", ksb_trivial (cfunU push_body))
+  Definition StackSbtb: list (gname * fspecbody) :=
+    [("new", mk_specbody fspec_trivial (cfunU new_body));
+    ("pop", mk_specbody fspec_trivial (cfunU pop_body));
+    ("push", mk_specbody fspec_trivial (cfunU push_body))
     ].
 
   Definition StackStb: list (gname * fspec).
     eapply (Seal.sealing "stb").
-    let x := constr:(List.map (map_snd (fun ksb => ksb.(ksb_fspec): fspec)) StackSbtb) in
+    let x := constr:(List.map (map_snd (fun fsb => fsb.(fsb_fspec): fspec)) StackSbtb) in
     let y := eval cbn in x in
     eapply y.
   Defined.
 
-  Definition KStackSem: KModSem.t := {|
-    KModSem.fnsems := StackSbtb;
-    KModSem.mn := "Stack";
-    KModSem.initial_mr := ε;
-    KModSem.initial_st := (∅: gmap mblock (list val))↑;
+  Definition SStackSem: SModSem.t := {|
+    SModSem.fnsems := StackSbtb;
+    SModSem.initial_mr := ε;
+    SModSem.initial_st := (∅: gmap mblock (list val))↑;
+    (* SModSem.initial_st := tt↑; *)
   |}
   .
   Definition StackSem (stb: gname -> option fspec): ModSem.t :=
-    KModSem.transl_tgt stb KStackSem.
+    (SModSem.to_tgt stb) SStackSem.
 
 
 
-  Definition KStack: KMod.t := {|
-    KMod.get_modsem := fun _ => KStackSem;
-    KMod.sk := [("new", Gfun↑); ("pop", Gfun↑); ("push", Gfun↑)];
+  Definition SStack: SMod.t := {|
+    SMod.get_modsem := fun _ => SStackSem;
+    SMod.sk := [("new", Gfun↑); ("pop", Gfun↑); ("push", Gfun↑)];
   |}
   .
   Definition Stack (stb: Sk.t -> gname -> option fspec): Mod.t :=
-    KMod.transl_tgt stb KStack.
+    (SMod.to_tgt stb) SStack.
 
 End PROOF.
 Global Hint Unfold StackStb: stb.
