examples/stack/Stack2.v
@@ -19,8 +19,8 @@ Section PROOF.
   Context `{Σ: GRA.t}.
   Context `{@GRA.inG memRA Σ}.
 
-  Notation pget := (p0 <- trigger PGet;; `p0: (gmap mblock (list val)) <- p0↓ǃ;; Ret p0) (only parsing).
-  Notation pput p0 := (trigger (PPut p0↑)) (only parsing).
+  Notation sget := (p0 <- trigger sGet;; `p0: (gmap mblock (list val)) <- p0↓ǃ;; Ret p0) (only parsing).
+  Notation sput p0 := (trigger (sPut p0↑)) (only parsing).
 
   (* def new(): Ptr *)
   (*   let handle := Choose(Ptr); *)
@@ -32,10 +32,10 @@ Section PROOF.
     fun args =>
       _ <- (pargs [] args)?;;
       handle <- trigger (Choose _);;
-      stk_mgr0 <- pget;;
+      stk_mgr0 <- sget;;
       guarantee(stk_mgr0 !! handle = None);;;
       let stk_mgr1 := <[handle:=[]]> stk_mgr0 in
-      pput stk_mgr1;;;
+      sput stk_mgr1;;;
       Ret (Vptr handle 0)
   .
 
@@ -51,11 +51,11 @@ Section PROOF.
   Definition pop_body: list val -> itree Es val :=
     fun args =>
       handle <- (pargs [Tblk] args)?;;
-      stk_mgr0 <- pget;;
+      stk_mgr0 <- sget;;
       stk0 <- (stk_mgr0 !! handle)?;;
       match stk0 with
       | x :: stk1 =>
-        pput (<[handle:=stk1]> stk_mgr0);;;
+        sput (<[handle:=stk1]> stk_mgr0);;;
         Ret x
       | _ => Ret (Vint (- 1))
       end
@@ -69,16 +69,15 @@ Section PROOF.
   Definition push_body: list val -> itree Es val :=
     fun args =>
       '(handle, x) <- (pargs [Tblk; Tuntyped] args)?;;
-      stk_mgr0 <- pget;;
+      stk_mgr0 <- sget;;
       stk0 <- (stk_mgr0 !! handle)?;;
-      pput (<[handle:=(x :: stk0)]> stk_mgr0);;;
+      sput (<[handle:=(x :: stk0)]> stk_mgr0);;;
       Ret Vundef
   .
 
   Definition StackSem: ModSem.t := {|
     ModSem.fnsems := [("new", cfunU new_body); ("pop", cfunU pop_body); ("push", cfunU push_body)];
-    ModSem.mn := "Stack";
-    ModSem.initial_st := (∅: gmap mblock (list val))↑;
+    ModSem.init_st := (∅: gmap mblock (list val))↑;
   |}
   .
 
