examples/stack/Stack32proof.v
@@ -1,4 +1,4 @@
-Require Import Stack2 Stack3A HoareDef SimModSem.
+Require Import Stack2 Stack3A HoareDef SimModSem SimModSemFacts.
 Require Import Coqlib.
 Require Import ImpPrelude.
 Require Import Skeleton.
@@ -23,56 +23,39 @@ Set Implicit Arguments.
 Local Open Scope nat_scope.
 
 
-
 Section REFINE.
   Context `{Σ: GRA.t}.
   Context `{@GRA.inG stkRA Σ}.
 
   Let W: Type := Any.t * Any.t.
 
-  Variable frds: Sk.t -> list string.
-
   Let wf: _ -> W -> Prop :=
     fun (_: unit) '(st_src, st_tgt) =>
       exists (st: gmap mblock (list val)),
         st_src = st↑ /\ st_tgt = st↑.
 
-  Theorem correct: refines2 [KMod.transl_src frds Stack3A.KStack] [Stack2.Stack].
+  Theorem correct: refines2 [SMod.to_src Stack3A.SStack] [Stack2.Stack].
   Proof.
     eapply adequacy_local2. econs; ss. i.
     econstructor 1 with (wf:=wf) (le:=top2); ss.
     2: { esplits; et. ss. }
     econs; ss.
-    { init. unfold Stack2.new_body, new_body, body_to_src.
-      red in WF. des; clarify.
-      match goal with
-      | |- context[my_if ?cond _ _] => destruct cond
-      end.
-      { steps. }
-      { steps. force_l. eexists. steps. force_l; et.
-        steps. red. esplits; et. red. esplits; et. }
+    { init. unfold cfunU, fun_to_src, Stack2.new_body, new_body, body_to_src.
+      red in WF. des; clarify. steps. force_l. eexists. steps. force_l; et.
+      steps. red. esplits; et. red. esplits; et.  
     }
     econs; ss.
-    { init. unfold Stack2.pop_body, pop_body, body_to_src.
+    { init. unfold cfunU, fun_to_src, Stack2.pop_body, pop_body, body_to_src.
       red in WF. des; clarify.
-      match goal with
-      | |- context[my_if ?cond _ _] => destruct cond
-      end.
-      { steps. }
-      { steps. rewrite _UNWRAPU1. steps. des_ifs.
-        { steps. red. esplits; et. red. esplits; et. }
-        { steps. red. esplits; et. red. esplits; et. }
-      }
+      steps. rewrite _UNWRAPU1. steps. des_ifs.
+      { steps. red. esplits; et. red. esplits; et. }
+      { steps. red. esplits; et. red. esplits; et. }
     }
     econs; ss.
-    { init. unfold Stack2.push_body, push_body, body_to_src.
+    { init. unfold cfunU, fun_to_src, Stack2.push_body, push_body, body_to_src.
       red in WF. des; clarify.
-      match goal with
-      | |- context[my_if ?cond _ _] => destruct cond
-      end.
-      { steps. }
-      { steps. rewrite _UNWRAPU0. steps.
-        red. esplits; et. red. esplits; et. }
+      steps. rewrite _UNWRAPU0. steps.
+      red. esplits; et. red. esplits; et. 
     }
     Unshelve. all: try exact 0. all: ss.
   Qed.
